proofs/fstar/extraction/Libcrux.Kem.Kyber.Hash_functions.fst
@@ -10,28 +10,34 @@ let v_H (input: t_Slice u8) = Libcrux.Digest.sha3_256_ input
 let v_PRF (v_LEN: usize) (input: t_Slice u8) = Libcrux.Digest.shake256 v_LEN input
 
 let v_XOF_absorb (v_K: usize) (input: t_Array (t_Array u8 (sz 34)) v_K) =
-  let state:Libcrux.Digest.t_Shake128State v_K = Libcrux.Digest.shake128_init v_K () in
-  let state:Libcrux.Digest.t_Shake128State v_K =
+  let state:t_Array Libcrux.Digest.t_Shake128State v_K =
+    Libcrux.Digest.impl__Shake128State__new v_K ()
+  in
+  let state:t_Array Libcrux.Digest.t_Shake128State v_K =
     Libcrux.Digest.shake128_absorb_final v_K state input
   in
   state
 
-let v_XOF_free (v_K: usize) (xof_state: Libcrux.Digest.t_Shake128State v_K) =
-  let xof_state:Libcrux.Digest.t_Shake128State v_K = Libcrux.Digest.impl_3__free v_K xof_state in
+let v_XOF_free (v_K: usize) (xof_state: t_Array Libcrux.Digest.t_Shake128State v_K) =
+  let _:Prims.unit = Libcrux.Digest.shake128_free v_K xof_state in
   ()
 
-let v_XOF_squeeze_block (v_K: usize) (xof_state: Libcrux.Digest.t_Shake128State v_K) =
-  let tmp0, out:(Libcrux.Digest.t_Shake128State v_K & t_Array (t_Array u8 (sz 168)) v_K) =
+let v_XOF_squeeze_block (v_K: usize) (xof_state: t_Array Libcrux.Digest.t_Shake128State v_K) =
+  let tmp0, out:(t_Array Libcrux.Digest.t_Shake128State v_K & t_Array (t_Array u8 (sz 168)) v_K) =
     Libcrux.Digest.shake128_squeeze_nblocks (sz 168) v_K xof_state
   in
-  let xof_state:Libcrux.Digest.t_Shake128State v_K = tmp0 in
+  let xof_state:t_Array Libcrux.Digest.t_Shake128State v_K = tmp0 in
   let output:t_Array (t_Array u8 (sz 168)) v_K = out in
-  output, xof_state <: (t_Array (t_Array u8 (sz 168)) v_K & Libcrux.Digest.t_Shake128State v_K)
+  output, xof_state
+  <:
+  (t_Array (t_Array u8 (sz 168)) v_K & t_Array Libcrux.Digest.t_Shake128State v_K)
 
-let v_XOF_squeeze_three_blocks (v_K: usize) (xof_state: Libcrux.Digest.t_Shake128State v_K) =
-  let tmp0, out:(Libcrux.Digest.t_Shake128State v_K & t_Array (t_Array u8 (sz 504)) v_K) =
+let v_XOF_squeeze_three_blocks (v_K: usize) (xof_state: t_Array Libcrux.Digest.t_Shake128State v_K) =
+  let tmp0, out:(t_Array Libcrux.Digest.t_Shake128State v_K & t_Array (t_Array u8 (sz 504)) v_K) =
     Libcrux.Digest.shake128_squeeze_nblocks (sz 504) v_K xof_state
   in
-  let xof_state:Libcrux.Digest.t_Shake128State v_K = tmp0 in
+  let xof_state:t_Array Libcrux.Digest.t_Shake128State v_K = tmp0 in
   let output:t_Array (t_Array u8 (sz 504)) v_K = out in
-  output, xof_state <: (t_Array (t_Array u8 (sz 504)) v_K & Libcrux.Digest.t_Shake128State v_K)
+  output, xof_state
+  <:
+  (t_Array (t_Array u8 (sz 504)) v_K & t_Array Libcrux.Digest.t_Shake128State v_K)
