proofs/fstar/extraction/Libcrux.Kem.Kyber.Sampling.fst
@@ -314,14 +314,14 @@ let sample_from_xof (v_K: usize) (seeds: t_Array (t_Array u8 (sz 34)) v_K) =
     Libcrux.Kem.Kyber.Arithmetic.t_PolynomialRingElement v_K =
     Rust_primitives.Hax.repeat Libcrux.Kem.Kyber.Arithmetic.impl__PolynomialRingElement__ZERO v_K
   in
-  let xof_state:Libcrux.Digest.t_Shake128State v_K =
+  let xof_state:t_Array Libcrux.Digest.t_Shake128State v_K =
     Libcrux.Kem.Kyber.Hash_functions.v_XOF_absorb v_K seeds
   in
-  let randomness, new_state:(t_Array (t_Array u8 (sz 504)) v_K & Libcrux.Digest.t_Shake128State v_K)
-  =
+  let randomness, new_state:(t_Array (t_Array u8 (sz 504)) v_K &
+    t_Array Libcrux.Digest.t_Shake128State v_K) =
     Libcrux.Kem.Kyber.Hash_functions.v_XOF_squeeze_three_blocks v_K xof_state
   in
-  let xof_state:Libcrux.Digest.t_Shake128State v_K = new_state in
+  let xof_state:t_Array Libcrux.Digest.t_Shake128State v_K = new_state in
   let tmp0, tmp1, out1:(t_Array usize v_K &
     t_Array Libcrux.Kem.Kyber.Arithmetic.t_PolynomialRingElement v_K &
     bool) =
@@ -333,31 +333,31 @@ let sample_from_xof (v_K: usize) (seeds: t_Array (t_Array u8 (sz 34)) v_K) =
   let done, out, sampled_coefficients, xof_state:(bool &
     t_Array Libcrux.Kem.Kyber.Arithmetic.t_PolynomialRingElement v_K &
     t_Array usize v_K &
-    Libcrux.Digest.t_Shake128State v_K) =
+    t_Array Libcrux.Digest.t_Shake128State v_K) =
     Rust_primitives.f_while_loop (fun temp_0_ ->
           let done, out, sampled_coefficients, xof_state:(bool &
             t_Array Libcrux.Kem.Kyber.Arithmetic.t_PolynomialRingElement v_K &
             t_Array usize v_K &
-            Libcrux.Digest.t_Shake128State v_K) =
+            t_Array Libcrux.Digest.t_Shake128State v_K) =
             temp_0_
           in
           ~.done <: bool)
       (done, out, sampled_coefficients, xof_state
         <:
         (bool & t_Array Libcrux.Kem.Kyber.Arithmetic.t_PolynomialRingElement v_K & t_Array usize v_K &
-          Libcrux.Digest.t_Shake128State v_K))
+          t_Array Libcrux.Digest.t_Shake128State v_K))
       (fun temp_0_ ->
           let done, out, sampled_coefficients, xof_state:(bool &
             t_Array Libcrux.Kem.Kyber.Arithmetic.t_PolynomialRingElement v_K &
             t_Array usize v_K &
-            Libcrux.Digest.t_Shake128State v_K) =
+            t_Array Libcrux.Digest.t_Shake128State v_K) =
             temp_0_
           in
           let randomness, new_state:(t_Array (t_Array u8 (sz 168)) v_K &
-            Libcrux.Digest.t_Shake128State v_K) =
+            t_Array Libcrux.Digest.t_Shake128State v_K) =
             Libcrux.Kem.Kyber.Hash_functions.v_XOF_squeeze_block v_K xof_state
           in
-          let xof_state:Libcrux.Digest.t_Shake128State v_K = new_state in
+          let xof_state:t_Array Libcrux.Digest.t_Shake128State v_K = new_state in
           let tmp0, tmp1, out1:(t_Array usize v_K &
             t_Array Libcrux.Kem.Kyber.Arithmetic.t_PolynomialRingElement v_K &
             bool) =
@@ -371,7 +371,7 @@ let sample_from_xof (v_K: usize) (seeds: t_Array (t_Array u8 (sz 34)) v_K) =
           <:
           (bool & t_Array Libcrux.Kem.Kyber.Arithmetic.t_PolynomialRingElement v_K &
             t_Array usize v_K &
-            Libcrux.Digest.t_Shake128State v_K))
+            t_Array Libcrux.Digest.t_Shake128State v_K))
   in
   let _:Prims.unit = Libcrux.Kem.Kyber.Hash_functions.v_XOF_free v_K xof_state in
   let _:Prims.unit = () <: Prims.unit in
