proofs/fstar/extraction/Libcrux.Digest.fsti
@@ -12,21 +12,21 @@ val sha3_512_ (payload: t_Slice u8)
 val shake256 (v_LEN: usize) (data: t_Slice u8)
     : Prims.Pure (t_Array u8 v_LEN) Prims.l_True (fun _ -> Prims.l_True)
 
-val t_Shake128State (v_K: usize) : Type
+val t_Shake128State:Type
 
-val impl_3__free (v_K: usize) (self: t_Shake128State v_K)
-    : Prims.Pure (t_Shake128State v_K) Prims.l_True (fun _ -> Prims.l_True)
+val impl__Shake128State__new: v_K: usize -> Prims.unit
+  -> Prims.Pure (t_Array t_Shake128State v_K) Prims.l_True (fun _ -> Prims.l_True)
 
 val shake128_absorb_final
       (v_K: usize)
-      (st: t_Shake128State v_K)
+      (st: t_Array t_Shake128State v_K)
       (data: t_Array (t_Array u8 (sz 34)) v_K)
-    : Prims.Pure (t_Shake128State v_K) Prims.l_True (fun _ -> Prims.l_True)
+    : Prims.Pure (t_Array t_Shake128State v_K) Prims.l_True (fun _ -> Prims.l_True)
 
-val shake128_init: v_K: usize -> Prims.unit
-  -> Prims.Pure (t_Shake128State v_K) Prims.l_True (fun _ -> Prims.l_True)
+val shake128_free (v_K: usize) (state: t_Array t_Shake128State v_K)
+    : Prims.Pure (t_Array t_Shake128State v_K) Prims.l_True (fun _ -> Prims.l_True)
 
-val shake128_squeeze_nblocks (v_OUTPUT_BYTES v_K: usize) (st: t_Shake128State v_K)
-    : Prims.Pure (t_Shake128State v_K & t_Array (t_Array u8 v_OUTPUT_BYTES) v_K)
+val shake128_squeeze_nblocks (v_OUTPUT_BYTES v_K: usize) (st: t_Array t_Shake128State v_K)
+    : Prims.Pure (t_Array t_Shake128State v_K & t_Array (t_Array u8 v_OUTPUT_BYTES) v_K)
       Prims.l_True
       (fun _ -> Prims.l_True)
